Change definition names: now globfun_weak_lsim rather than fundef_weak_lsim.

diff.py
@@ -3,7 +3,15 @@
 import os, subprocess
 
 if __name__ == "__main__":
-    for passname in ["Renumber", "Constprop", "Deadcode", "CSE", "Tailcall", "Inlining"]:
-        output1 = subprocess.check_output("diff ../backend/%sproof.v backend/%sproof_linker.v | grep \"^>\" | wc -l" % (passname, passname), shell=True)
-        output2 = subprocess.check_output("diff ../backend/%sproof.v backend/%sproof_linker.v | grep \"^> (\*\" | wc -l" % (passname, passname), shell=True)
+    s1 = 0
+    s2 = 0
+    s3 = 0
+    for passname in ["Renumberproof", "Constpropproof", "Deadcodeproof", "CSEproof", "Tailcallproof", "Inliningproof", "Selectionproof", "SimplExprproof", "ValueAnalysis"]:
+        output1 = subprocess.check_output("diff ../*/%s.v */%s_linker.v | grep \"^>\" | wc -l" % (passname, passname), shell=True)
+        output2 = subprocess.check_output("diff ../*/%s.v */%s_linker.v | grep \"^> (\*\" | wc -l" % (passname, passname), shell=True)
         print("%s:\t%d \t- 1.5*%d \t= %d" % (passname, int(output1), int(output2), int(int(output1) - int(output2) * 1.5)))
+        s1 += int(output1)
+        s2 += int(output2)
+        s3 += int(int(output1) - int(output2) * 1.5)
+    print("")
+    print("%s:\t%d \t- 1.5*%d \t= %d" % ("\tTotal", s1, s2, s3))
