backend/Constpropproof_linker.v
@@ -45,11 +45,6 @@ Hypothesis (Hfsim: @program_weak_lsim Language_RTL Language_RTL transf_sigT tran
 Hypothesis (Hfprog: program_linkeq Language_RTL prog fprog).
 Hypothesis (Hftprog: program_linkeq Language_RTL tprog ftprog).
 
-Let globfun_weak_lsim :=
-  @globfun_lsim Language_RTL Language_RTL transf_sigT transf_efT
-                (fun _ _ _ _ => True)
-                fprog ftprog.
-
 Let ge := Genv.globalenv fprog.
 Let tge := Genv.globalenv ftprog.
 
@@ -61,7 +56,7 @@ Lemma transf_ros_correct:
   regs_lessdef rs rs' ->
   exists f',
   find_function tge (transf_ros ae ros) rs' = Some f' /\
-  fundef_weak_lsim Language_RTL Language_RTL transf_sigT ge tge f f'.
+  globfun_weak_lsim Language_RTL Language_RTL transf_sigT ge tge f f'.
 Proof.
   intros until rs'; intros GE EM FF RLD.
   eapply find_function_translated_Constprop; eauto.
@@ -140,7 +135,7 @@ Inductive match_call: nat -> state -> state -> Prop :=
   | match_states_call:
       forall s f args m s' f' args' m'
            (STACKS: list_forall2 match_stackframes s s')
-           (FUN: fundef_weak_lsim Language_RTL Language_RTL transf_sigT ge tge f f')
+           (FUN: globfun_weak_lsim Language_RTL Language_RTL transf_sigT ge tge f f')
            (ARGS: Val.lessdef_list args args')
            (MEM: Mem.extends m m'),
       match_call O (Callstate s f args m)
